lib/pulse/lib/Pulse.Lib.HigherArray.fst
@@ -33,151 +33,470 @@ module PA = Pulse.Lib.PCM.Array
 /// An abstract type to represent a base array (whole allocation
 /// unit), exposed for proof purposes only
 [@@erasable]
-let base_t
-: Type0
-= Ghost.erased (SZ.t & core_pcm_ref)
-
-let base_len (b: base_t) : GTot nat = SZ.v (fst b)
-
-/// An abstract type to represent a C pointer, as a base and an offset
-/// into its base
-let l_pcm_ref (elt:Type u#a) (base_len:SZ.t) =
-  r:pcm_ref (PA.pcm elt (SZ.v base_len)){ 
-      r =!= null_core_pcm_ref \/
-      base_len = 0sz
-  }
-
-
-noeq
-type ptr : Type0 = {
-  base_len: Ghost.erased SZ.t;
-  base: (base:core_pcm_ref { base == null_core_pcm_ref ==> SZ.v base_len == 0});
-  offset: (offset: nat { offset <= SZ.v base_len });
+noeq type base_t : Type0 = {
+  base_len: base_len:nat { SZ.fits base_len };
+  base_ref: base_ref:core_pcm_ref {
+    base_ref == null_core_pcm_ref ==> base_len == 0
+  };
 }
 
-
-let null_ptr
-: ptr
-= { base_len = 0sz; base = null_core_pcm_ref ; offset = 0 }
-
-
-let is_null_ptr (p:ptr)
-: Pure bool
-  (requires True)
-  (ensures (fun res -> res == true <==> p == null_ptr))
-= is_null_core_pcm_ref p.base
-
-let base (p: ptr)
-: Tot base_t
-= ( Ghost.reveal p.base_len, p.base )
-
-let offset (p: ptr)
-: Ghost nat (requires True) (ensures (fun offset -> offset <= base_len (base p)))
-= p.offset
-
-let ptr_base_offset_inj (p1 p2: ptr) : Lemma
-  (requires (
-    base p1 == base p2 /\
-    offset p1 == offset p2
-  ))
-  (ensures (
-    p1 == p2
-  ))
-= ()
-
-let base_len_null_ptr : squash  (base_len (base (null_ptr)) == 0)
-= ()
-
 noeq
-type array'
-: Type0
-= { p: ptr;
-    length: (l:Ghost.erased nat {offset p + l <= base_len (base p)})
-  }
-let array ([@@@strictly_positive] elt: Type u#1) : Type0 = array'
+type array' : Type0 = {
+  base_len: base_len:Ghost.erased nat { SZ.fits base_len };
+  base_ref: base_ref:core_pcm_ref {
+    base_ref == null_core_pcm_ref ==> base_len == hide 0
+  };
+  offset: offset: nat { offset <= base_len };
+  length: length:Ghost.erased nat {offset + length <= base_len };
+}
+let array elt = array'
+
+let null_array' : array' = { base_len = 0; base_ref = null_core_pcm_ref; offset = 0; length = 0 }
 
 let length (#elt: Type) (a: array elt) = a.length
-
-let ptr_of
-  (#elt: Type)
-  (a: array elt)
-: Tot (ptr)
-= a.p
+let base_of #t (a: array t) : base_t = { base_len = a.base_len; base_ref = a.base_ref }
+let offset_of #t (a: array t) : GTot nat = a.offset
 
 let is_full_array (#elt: Type) (a: array elt) : Tot prop =
-  length a == base_len (base (ptr_of a))
+  length a == reveal a.base_len
 
-let null (#a: Type u#1) : array a
-= { p = null_ptr; length =Ghost.hide 0 }
-let is_null a = is_null_ptr a.p
+let null (#a: Type u#1) : array a = null_array'
+let is_null a = is_null_core_pcm_ref a.base_ref
 
-let length_fits #elt a = ()
+let lptr_of #elt (a: array elt) : pcm_ref (PA.pcm elt a.base_len) =
+  a.base_ref
 
-let valid_perm
-  (len: nat)
-  (offset: nat)
-  (slice_len: nat)
-  (p: perm)
-: prop
-= let open FStar.Real in
-  ((offset + slice_len <= len /\ slice_len > 0) ==> (p <=. one))
+let mk_carrier_f #elt (off: nat) (len: nat) (f: perm) (v: Seq.seq elt) (mask: nat -> bool) :
+    index_t len -> Pulse.Lib.PCM.Fraction.fractional elt = fun i ->
+  if off <= i && i < off + Seq.length v && mask (i - off) then
+    Some (Seq.index v (i - off), f)
+  else
+    None
 
-let l_pcm_ref' (elt:Type u#a) (base_len:SZ.t) =
-  r:pcm_ref (PA.pcm elt (SZ.v base_len))
+let mk_carrier #elt (off: nat) (len: nat) (f: perm) (v: Seq.seq elt) (mask: nat -> bool) : carrier elt len =
+  Map.map_literal #(index_t len) #(Pulse.Lib.PCM.Fraction.fractional elt) (mk_carrier_f off len f v mask)
 
-let lptr_of (#elt:Type u#1) (a:array elt)
-  : Tot (l_pcm_ref elt ( (ptr_of a).base_len))
-  = (ptr_of a).base
+irreducible let pull_mask (f: nat -> prop) (len: nat) : Ghost (nat -> bool) (requires True)
+    (ensures fun res -> forall i. res i <==> i >= len \/ f i) =
+  let s = Seq.init_ghost len fun i -> IndefiniteDescription.strong_excluded_middle (f i) in
+  fun i -> if i < len then Seq.index s i else true
+
+let mk_carrier' #t (a: array t) (f: perm) (v: Seq.seq t) (mask: nat -> prop) : GTot (carrier t a.base_len) =
+  mk_carrier a.offset a.base_len f v (pull_mask mask a.length)
+
+let mask_nonempty (mask: nat -> prop) (len: nat) : prop =
+  exists i. mask i /\ i < len
+
+// workaround for https://github.com/FStarLang/pulse/issues/430
+let squash' (t: Type u#1) = squash t
+
+let pts_to_mask #t ([@@@mkey] a: array t) (#[full_default()] f: perm) (v: erased (Seq.seq t)) (mask: nat -> prop) : slprop =
+  pcm_pts_to (lptr_of a) (mk_carrier' a f v mask) **
+  pure (Seq.length v == reveal a.length /\ (mask_nonempty mask a.length ==> f <=. 1.0R) /\ squash' t)
+
+let pts_to_mask_timeless _ _ _ _ = ()
+
+ghost
+fn pts_to_mask_props #t (a:array t) (#p:perm) (#x:Seq.seq t) #mask
+  preserves pts_to_mask a #p x mask
+  ensures pure (length a == Seq.length x)
+  ensures pure (mask_nonempty mask (length a) ==> p <=. 1.0R)
+  ensures pure (~(is_null a))
+  ensures pure (squash' t)
+{
+  unfold pts_to_mask a #p x mask;
+  pts_to_not_null _ _;
+  fold pts_to_mask a #p x mask;
+}
+
+ghost
+fn pts_to_mask_len #t (a:array t) (#p:perm) (#x:Seq.seq t) #mask
+  preserves pts_to_mask a #p x mask
+  ensures pure (length a == Seq.length x)
+{
+  pts_to_mask_props a;
+}
+
+ghost
+fn pts_to_mask_not_null #a #p (r:array a) (#v:Seq.seq a) #mask
+  preserves pts_to_mask r #p v mask
+  ensures pure (not (is_null r))
+{
+  pts_to_mask_props r;
+}
+
+ghost fn mask_vext #t (arr: array t) #f #v v' #mask
+  requires pts_to_mask arr #f v mask
+  requires pure (Seq.length v' == Seq.length v /\
+    (forall (i: nat). mask i /\ i < Seq.length v ==> Seq.index v i == Seq.index v' i))
+  ensures pts_to_mask arr #f v' mask
+{
+  unfold pts_to_mask arr #f v mask;
+  assert pure (mk_carrier' arr f v mask `Map.equal` mk_carrier' arr f v' mask);
+  fold pts_to_mask arr #f v' mask;
+}
+
+ghost fn mask_mext #t (arr: array t) #f #v #mask (mask': nat -> prop)
+  requires pts_to_mask arr #f v mask
+  requires pure (forall (i: nat). i < Seq.length v ==> (mask i <==> mask' i))
+  ensures pts_to_mask arr #f v mask'
+{
+  unfold pts_to_mask arr #f v mask;
+  assert pure (mk_carrier' arr f v mask `Map.equal` mk_carrier' arr f v mask');
+  fold pts_to_mask arr #f v mask';
+}
+
+ghost fn mask_ext #t (arr: array t) #f #v #mask v' (mask': nat -> prop)
+  requires pts_to_mask arr #f v mask
+  requires pure (forall (i: nat). i < Seq.length v ==> (mask i <==> mask' i))
+  requires pure (Seq.length v' == Seq.length v /\
+    (forall (i: nat). mask i /\ i < Seq.length v ==> Seq.index v i == Seq.index v' i))
+  ensures pts_to_mask arr #f v' mask'
+{
+  mask_vext arr v';
+  mask_mext arr mask';
+}
+
+let get_mask_idx (m: nat->prop) (l: nat) : GTot (i: nat { mask_nonempty m l ==> i < l /\ m i }) =
+  if IndefiniteDescription.strong_excluded_middle (mask_nonempty m l) then
+    IndefiniteDescription.indefinite_description_ghost nat fun i -> i < l /\ m i
+  else
+    0
+
+ghost fn pcm_rw #t
+    (a1: array t) p1 s1 m1
+    (a2: array t) p2 s2 m2
+  requires pts_to_mask #t a1 #p1 s1 m1
+  requires pure (
+    a1.base_len == a2.base_len /\
+    a1.base_ref == a2.base_ref /\
+    reveal a2.length == Seq.length s2 /\
+    mk_carrier' a1 p1 s1 m1 `Map.equal` mk_carrier' a2 p2 s2 m2
+  )
+  ensures pts_to_mask #t a2 #p2 s2 m2
+{
+  unfold pts_to_mask a1 #p1 s1 m1;
+  rewrite each lptr_of a1 as lptr_of a2;
+  let i = get_mask_idx m2 (length a2);
+  assert pure (mask_nonempty m2 (length a2) ==>
+    Map.sel (mk_carrier' a2 p2 s2 m2) (i + a2.offset) == Some (Seq.index s2 i, p2));
+  fold pts_to_mask a2 #p2 s2 m2;
+}
+
+ghost fn pcm_share #t
+    (a: array t) p s m
+    (a1: array t) p1 s1 m1
+    (a2: array t) p2 s2 m2
+  requires pts_to_mask a #p s m
+  requires pure (Seq.length s1 == a1.length)
+  requires pure (Seq.length s2 == a2.length)
+  requires pure (
+    a1.base_len == a.base_len /\ a2.base_len == a.base_len /\
+    a1.base_ref == a.base_ref /\ a2.base_ref == a.base_ref /\
+    composable (mk_carrier' a1 p1 s1 m1) (mk_carrier' a2 p2 s2 m2) /\
+    compose (mk_carrier' a1 p1 s1 m1) (mk_carrier' a2 p2 s2 m2)
+      `Map.equal` mk_carrier' a p s m
+  )
+  ensures pts_to_mask a1 #p1 s1 m1
+  ensures pts_to_mask a2 #p2 s2 m2
+{
+  unfold pts_to_mask a #p s m;
+  Pulse.Lib.Core.share (lptr_of a) (mk_carrier' a1 p1 s1 m1) (mk_carrier' a2 p2 s2 m2);
+  rewrite
+    pcm_pts_to (lptr_of a) (mk_carrier' a1 p1 s1 m1) as
+    pcm_pts_to (lptr_of a1) (mk_carrier' a1 p1 s1 m1);
+  rewrite
+    pcm_pts_to (lptr_of a) (mk_carrier' a2 p2 s2 m2) as
+    pcm_pts_to (lptr_of a2) (mk_carrier' a2 p2 s2 m2);
+  let i1 = get_mask_idx m1 (length a1);
+  let i2 = get_mask_idx m2 (length a2);
+  assert pure (mask_nonempty m1 (length a1) ==>
+    Some? (Map.sel (mk_carrier' a p s m) (i1 + a1.offset)));
+  fold pts_to_mask a1 #p1 s1 m1;
+  assert pure (mask_nonempty m2 (length a2) ==>
+    Some? (Map.sel (mk_carrier' a p s m) (i2 + a2.offset)));
+  fold pts_to_mask a2 #p2 s2 m2;
+}
+
+ghost fn pcm_gather #t
+    (a: array t) p s m
+    (a1: array t) p1 s1 m1
+    (a2: array t) p2 s2 m2
+  requires pure (Seq.length s == a.length)
+  requires pure (
+    a1.base_len == a.base_len /\ a2.base_len == a.base_len /\
+    a1.base_ref == a.base_ref /\ a2.base_ref == a.base_ref /\
+    (composable (mk_carrier' a1 p1 s1 m1) (mk_carrier' a2 p2 s2 m2) ==>
+    compose (mk_carrier' a1 p1 s1 m1) (mk_carrier' a2 p2 s2 m2)
+      `Map.equal` mk_carrier' a p s m)
+  )
+  requires pts_to_mask a1 #p1 s1 m1
+  requires pts_to_mask a2 #p2 s2 m2
+  ensures pts_to_mask a #p s m
+  ensures pure (
+    a1.base_len == a.base_len /\ a2.base_len == a.base_len /\
+    a1.base_ref == a.base_ref /\ a2.base_ref == a.base_ref /\
+    composable (mk_carrier' a1 p1 s1 m1) (mk_carrier' a2 p2 s2 m2) /\
+    compose (mk_carrier' a1 p1 s1 m1) (mk_carrier' a2 p2 s2 m2)
+      `Map.equal` mk_carrier' a p s m
+  )
+{
+  unfold pts_to_mask a1 #p1 s1 m1;
+  unfold pts_to_mask a2 #p2 s2 m2;
+  rewrite
+    pcm_pts_to (lptr_of a1) (mk_carrier' a1 p1 s1 m1) as
+    pcm_pts_to (lptr_of a) (mk_carrier' a1 p1 s1 m1);
+  rewrite
+    pcm_pts_to (lptr_of a2) (mk_carrier' a2 p2 s2 m2) as
+    pcm_pts_to (lptr_of a) (mk_carrier' a2 p2 s2 m2);
+  Pulse.Lib.Core.gather (lptr_of a) (mk_carrier' a1 p1 s1 m1) (mk_carrier' a2 p2 s2 m2);
+  let i = get_mask_idx m (length a);
+  assert pure (mask_nonempty m a.length ==>
+    Map.sel (mk_carrier' a p s m) (i + a.offset) == Some (Seq.index s i, p));
+  fold pts_to_mask a #p s m;
+}
+
+ghost
+fn mask_share #a (arr:array a) (#s: Seq.seq a) #p #mask
+  requires pts_to_mask arr #p s mask
+  ensures pts_to_mask arr #(p /. 2.0R) s mask
+  ensures pts_to_mask arr #(p /. 2.0R) s mask
+{
+  pts_to_mask_props arr;
+  pcm_share
+    arr p s mask
+    arr (p /. 2.0R) s mask
+    arr (p /. 2.0R) s mask;
+}
+
+[@@allow_ambiguous]
+ghost fn mask_gather #t (arr: array t) #p1 #p2 #s1 #s2 #mask1 #mask2
+  requires pts_to_mask arr #p1 s1 mask1
+  requires pts_to_mask arr #p2 s2 mask2
+  requires pure (forall i. mask1 i <==> mask2 i)
+  ensures exists* (v: Seq.seq t). pts_to_mask arr #(p1 +. p2) v mask1 **
+    pure ((Seq.length v == Seq.length s1 /\ Seq.length v == Seq.length s2) /\
+      (forall (i: nat). i < Seq.length v /\ mask1 i ==> Seq.index v i == Seq.index s1 i /\ Seq.index v i == Seq.index s2 i))
+{
+  mask_mext arr #p2 #s2 mask1;
+  pts_to_mask_props arr #p1 #s1 #mask1;
+  pts_to_mask_props arr #p2 #s2 #mask1;
+  pcm_gather
+    arr (p1 +. p2) s1 mask1
+    arr p1 s1 mask1
+    arr p2 s2 mask1;
+  assert pure (forall (i: nat). (i < Seq.length s1 /\ mask1 i) ==>
+    Map.sel (mk_carrier' arr p1 s1 mask1) (i + arr.offset) == Some (Seq.index s1 i, p1));
+}
+
+ghost fn split_mask #t (arr: array t) #f #v #mask (pred: nat -> prop)
+  requires pts_to_mask arr #f v mask
+  ensures pts_to_mask arr #f v (mask_isect mask pred)
+  ensures pts_to_mask arr #f v (mask_diff mask pred)
+{
+  pts_to_mask_props arr;
+  pcm_share
+    arr f v mask
+    arr f v (mask_isect mask pred)
+    arr f v (mask_diff mask pred);
+}
+
+let mix #t (v1: Seq.seq t) (v2: Seq.seq t { Seq.length v1 == Seq.length v2 }) (mask: nat -> prop) :
+    GTot (res: Seq.seq t { Seq.length res == Seq.length v1 /\
+      (forall (i: nat). i < Seq.length res ==>
+        (mask i ==> Seq.index res i == Seq.index v1 i) /\
+        (~(mask i) ==> Seq.index res i == Seq.index v2 i)) }) =
+  Seq.init_ghost (Seq.length v1) fun i ->
+    if IndefiniteDescription.strong_excluded_middle (mask i) then Seq.index v1 i else Seq.index v2 i
+
+[@@allow_ambiguous]
+ghost fn join_mask #t (arr: array t) #f #v1 #v2 #mask1 #mask2
+  requires pts_to_mask arr #f v1 mask1
+  requires pts_to_mask arr #f v2 mask2
+  requires pure (forall i. ~(mask1 i /\ mask2 i))
+  ensures exists* (v: Seq.seq t).
+    pts_to_mask arr #f v (fun i -> mask1 i \/ mask2 i) **
+    pure (Seq.length v == Seq.length v1 /\ Seq.length v == Seq.length v2 /\
+      (forall (i: nat). i < Seq.length v ==>
+        (mask1 i ==> Seq.index v i == Seq.index v1 i) /\
+        (mask2 i ==> Seq.index v i == Seq.index v2 i)))
+{
+  pts_to_mask_props arr #f #v1 #mask1;
+  pts_to_mask_props arr #f #v2 #mask2;
+  let v = mix v1 v2 mask1;
+  with mask. assert pure (mask == (fun i -> mask1 i \/ mask2 i));
+  pcm_gather
+    arr f v mask
+    arr f v1 mask1
+    arr f v2 mask2;
+}
+
+[@@allow_ambiguous]
+ghost fn join_mask' #t (arr: array t) #f (#v: erased (Seq.seq t)) #mask1 #mask2
+  requires pts_to_mask arr #f v mask1
+  requires pts_to_mask arr #f v mask2
+  requires pure (forall i. ~(mask1 i /\ mask2 i))
+  ensures pts_to_mask arr #f v (fun i -> mask1 i \/ mask2 i)
+{
+  join_mask arr #f #v #v #mask1 #mask2;
+  mask_vext arr v;
+}
+
+[@@allow_ambiguous]
+ghost
+fn pts_to_mask_injective_eq #a #p0 #p1 #s0 #s1 #mask0 #mask1 (arr:array a)
+  preserves pts_to_mask arr #p0 s0 mask0
+  preserves pts_to_mask arr #p1 s1 mask1
+  ensures pure (Seq.length s0 == Seq.length s1 /\
+    (forall (i: nat). i < Seq.length s0 /\ mask0 i /\ mask1 i ==>
+      Seq.index s0 i == Seq.index s1 i))
+{
+  unfold pts_to_mask arr #p0 s0 mask0;
+  unfold pts_to_mask arr #p1 s1 mask1;
+  Pulse.Lib.Core.gather (lptr_of arr) (mk_carrier' arr p0 s0 mask0) (mk_carrier' arr p1 s1 mask1);
+  Pulse.Lib.Core.share (lptr_of arr) (mk_carrier' arr p0 s0 mask0) (mk_carrier' arr p1 s1 mask1);
+  assert pure (forall (i: nat). i < Seq.length s0 /\ mask0 i ==>
+    Map.sel (mk_carrier' arr p0 s0 mask0) (i + arr.offset) == Some (Seq.index s0 i, p0));
+  fold pts_to_mask arr #p0 s0 mask0;
+  fold pts_to_mask arr #p1 s1 mask1;
+}
+
+fn mask_read #t (a: array t) (i: SZ.t) #p (#s: erased (Seq.seq t) { SZ.v i < Seq.length s }) #mask
+  preserves pts_to_mask a #p s mask
+  requires pure (mask (SZ.v i))
+  returns res: t
+  ensures pure (res == Seq.index s (SZ.v i))
+{
+  unfold pts_to_mask a #p s mask;
+  with w. assert pcm_pts_to (lptr_of a) w;
+  let v = Pulse.Lib.Core.read (lptr_of a) w (fun _ -> w);
+  fold pts_to_mask a #p s mask;
+  fst (Some?.v (FStar.Map.sel v (a.offset + SZ.v i)));
+}
+
+fn mask_write #t (a: array t) (i: SZ.t) (v: t) (#s: erased (Seq.seq t) { SZ.v i < Seq.length s }) #mask
+  requires pts_to_mask a s mask
+  requires pure (mask (SZ.v i))
+  ensures pts_to_mask a (Seq.upd s (SZ.v i) v) mask
+{
+  unfold pts_to_mask a s mask;
+  with w. assert (pcm_pts_to (lptr_of a) w);
+  Pulse.Lib.Core.write (lptr_of a) w _
+      (PM.lift_frame_preserving_upd
+        _ _
+        (Frac.mk_frame_preserving_upd
+          (Seq.index s (SZ.v i))
+          v
+        )
+        _ (a.offset + SZ.v i));
+  assert pure (
+    Map.upd (mk_carrier' a 1.0R s mask) (a.offset + SZ.v i) (Some (v, 1.0R))
+    `Map.equal`
+    mk_carrier' a 1.0R (Seq.upd s (SZ.v i) v) mask
+  );
+  fold pts_to_mask a (Seq.upd s (SZ.v i) v) mask;
+}
+
+let sub_impl #t (arr: array t) (i: nat) (j: erased nat { i <= j /\ j <= length arr }) : array t =
+  { arr with offset = arr.offset + i; length = j - i }
+
+let gsub #t (arr: array t) (i: nat) (j: nat { i <= j /\ j <= length arr }) : GTot (array t) =
+  sub_impl arr i j
+
+ghost fn gsub_intro #t (arr: array t) #f #mask (i j: nat) (#v: erased (Seq.seq t) { i <= j /\ j <= Seq.length v })
+  requires pts_to_mask arr #f v mask
+  requires pure (forall (k: nat). mask k ==> i <= k /\ k < j)
+  returns _: squash (length arr == Seq.length v)
+  ensures pts_to_mask (gsub arr i j) #f (Seq.slice v i j) (fun k -> mask (k + i))
+{
+  pts_to_mask_props arr;
+  pcm_rw
+    arr f v mask
+    (gsub arr i j) f (Seq.slice v i j) (fun k -> mask (k + i));
+  ()
+}
+
+let elim_squash (t: Type u#1 { squash' t }) : GTot t =
+  let h : squash (squash' t) = () in
+  let h : squash t = IndefiniteDescription.elim_squash h in
+  IndefiniteDescription.elim_squash h
+
+ghost fn gsub_elim #t (arr: array t) #f (#mask: nat->prop) (i j: nat)
+    (#v: erased (Seq.seq t) { i <= j /\ j <= length arr })
+  requires pts_to_mask (gsub arr i j) #f v mask
+  returns _: squash (j - i == Seq.length v)
+  ensures exists* v'.
+    pts_to_mask arr #f v' (fun k -> i <= k /\ k < j /\ mask (k - i)) **
+    pure (Seq.length v' == length arr /\ (forall (k:nat). k < j - i ==> Seq.index v k == Seq.index v' (k + i)))
+{
+  pts_to_mask_props (gsub arr i j);
+  let dummy = elim_squash t;
+  let v' = Seq.init_ghost (length arr) (fun k ->
+    if i <= k && k < j then Seq.index v (k - i) else dummy);
+  pcm_rw
+    (gsub arr i j) f v mask
+    arr f v' (fun k -> i <= k /\ k < j /\ mask (k - i));
+  ()
+}
+
+unobservable
+fn sub #t (arr: array t) #f #mask (i: SZ.t) (j: SZ.t)
+    (#v: erased (Seq.seq t) { SZ.v i <= SZ.v j /\ SZ.v j <= Seq.length (reveal v) })
+  requires pts_to_mask arr #f v mask
+  returns sub: (sub: array t { length arr == Seq.length (reveal v) })
+  ensures rewrites_to sub (gsub arr (SZ.v i) (SZ.v j))
+  ensures pts_to_mask sub #f (Seq.slice v (SZ.v i) (SZ.v j)) (fun k -> mask (k + SZ.v i))
+  ensures pts_to_mask arr #f v (fun k -> mask k /\ ~(SZ.v i <= k /\ k < SZ.v j))
+{
+  let pred = (fun k -> SZ.v i <= k /\ k < SZ.v j);
+  pts_to_mask_props arr;
+  split_mask arr pred;
+  gsub_intro arr #f #(mask_isect mask pred) (SZ.v i) (SZ.v j);
+  mask_mext (gsub arr (SZ.v i) (SZ.v j)) (fun k -> mask (k + SZ.v i));
+  rewrite each gsub arr (SZ.v i) (SZ.v j) as sub_impl arr (SZ.v i) (SZ.v j);
+  sub_impl arr (SZ.v i) (SZ.v j)
+}
+
+[@@allow_ambiguous]
+ghost fn return_sub #t (arr sub: array t) #f (#v #vsub: erased (Seq.seq t)) #mask #masksub (#i: nat) (#j: nat { i <= j /\ j <= length arr })
+  requires pts_to_mask arr #f v mask
+  requires pts_to_mask (gsub arr i j) #f vsub masksub
+  requires pure (forall (k: nat). i <= k /\ k < j ==> ~(mask k))
+  ensures exists* v'. pts_to_mask arr #f v' (fun k -> mask k \/ (i <= k /\ k < j /\ masksub (k - i)))
+    ** pure (Seq.length v == Seq.length v' /\ i + Seq.length vsub == j /\ j <= Seq.length v /\
+      (forall (k: nat). k < Seq.length v' ==>
+      Seq.index v' k == (if i <= k && k < j then Seq.index vsub (k - i) else Seq.index v k)))
+{
+  gsub_elim arr i j;
+  join_mask arr;
+  let v' = Seq.init_ghost (Seq.length v) (fun k -> 
+    if i <= k && k < j then Seq.index vsub (k - i) else Seq.index v k);
+  mask_ext arr v' (fun k -> mask k \/ (i <= k /\ k < j /\ masksub (k - i)));
+}
 
 let pts_to (#elt: Type u#1) (a: array elt) (#p: perm) (s: Seq.seq elt) : Tot slprop =
-  pcm_pts_to
-    (lptr_of a)
-    (mk_carrier (SZ.v (ptr_of a).base_len) (ptr_of a).offset s p) **
-  pure (
-    valid_perm (SZ.v (ptr_of a).base_len) (ptr_of a).offset (Seq.length s) p /\
-    Seq.length s == length a
-  )
+  pts_to_mask a #p s fun i -> True
+
+ghost fn to_mask #t (arr: array t) #f #v
+  requires arr |-> Frac f v
+  ensures pts_to_mask arr #f v (fun _ -> True)
+{
+  unfold pts_to arr #f v;
+}
+
+ghost fn from_mask #t (arr: array t) #f #v #mask
+  requires pts_to_mask arr #f v mask
+  requires pure (forall i. mask i)
+  ensures arr |-> Frac f v
+{
+  mask_mext arr (fun _ -> True);
+  fold pts_to arr #f v;
+}
 
 let pts_to_timeless _ _ _ = ()
 
-let mk_array
-    (#elt: Type u#1)
-    (base_len: SZ.t)
-    (base:l_pcm_ref elt base_len)
-    (offset:nat { offset <= SZ.v base_len})
-: array elt
-= { p = { base_len; base; offset} ; length = Ghost.hide (SZ.v base_len - offset) }
-
-
 ghost
-fn fold_pts_to
-    (#elt: Type u#1)
-    (base_len: SZ.t)
-    (base:l_pcm_ref elt base_len)
-    (offset:nat { offset <= SZ.v base_len})
-    (#p: perm { p <=. 1.0R})
-    (s: Seq.seq elt { Seq.length s == SZ.v base_len - offset})
-requires
-  pcm_pts_to base (mk_carrier (SZ.v base_len) offset s p)
-ensures
-  pts_to (mk_array base_len base offset) #p s
-{
-  let a = (mk_array base_len base offset);
-  rewrite (pcm_pts_to base (mk_carrier (SZ.v base_len) offset s p))
-      as pcm_pts_to (lptr_of a)
-            (mk_carrier (SZ.v (ptr_of a).base_len) 
-                        (ptr_of a).offset
-                        s p);
-  fold (pts_to a #p s);
-  rewrite (pts_to a #p s)
-        as (pts_to (mk_array base_len base offset) #p s);
-}
-
-
-
-
-ghost
-fn pts_to_len'
+fn pts_to_len
   (#elt: Type u#1)
   (a:array elt)
   (#p:perm)
@@ -186,11 +505,9 @@ fn pts_to_len'
   ensures pts_to a #p x ** pure (length a == Seq.length x)
 {
   unfold pts_to a #p x;
+  pts_to_mask_len a;
   fold pts_to a #p x;
 }
-
-let pts_to_len = pts_to_len'
-
 
 ghost
 fn pts_to_not_null (#a:_) (#p:_) (r:array a) (#v:Seq.seq a)
@@ -198,32 +515,33 @@ fn pts_to_not_null (#a:_) (#p:_) (r:array a) (#v:Seq.seq a)
   ensures  pure (not (is_null #a r))
 {
   unfold pts_to r #p v;
-  let res = pts_to_not_null #_ #(PA.pcm a (SizeT.v r.p.base_len)) r.p.base _;
+  pts_to_mask_not_null _;
   fold pts_to r #p v;
-  res
 }
 
+let intro_squash #t (x: t) : squash' t = ()
 
-fn alloc' 
+fn alloc
     (#elt: Type u#1)
     (x: elt)
     (n: SZ.t)
-  requires emp
   returns a:array elt
 ensures 
   pts_to a (Seq.create (SZ.v n) x) **
   pure (length a == SZ.v n /\ is_full_array a)
 {
-  let v = (mk_carrier (SZ.v n) 0 (Seq.create (SZ.v n) x) 1.0R);
+  let v = mk_carrier 0 (SZ.v n) 1.0R (Seq.create (SZ.v n) x) (fun _ -> true);
   FStar.PCM.compatible_refl (PA.pcm elt (SZ.v n)) v;
   let b = Pulse.Lib.Core.alloc #_ #(PA.pcm elt (SZ.v n)) v;
   Pulse.Lib.Core.pts_to_not_null b _;
-  fold_pts_to n b 0 #1.0R (Seq.create (SZ.v n) x);
-  mk_array n b 0;
+  let arr: array elt = { base_ref = b; base_len = SZ.v n; length = SZ.v n; offset = 0 };
+  rewrite each b as lptr_of arr;
+  assert pure (v `Map.equal` mk_carrier' arr 1.0R (Seq.create (SZ.v n) x) (fun _ -> l_True));
+  intro_squash x;
+  fold pts_to_mask arr (Seq.create (SZ.v n) x) (fun _ -> l_True);
+  fold pts_to arr (Seq.create (SZ.v n) x);
+  arr
 }
-
-let alloc = alloc'
-
 
 fn read
     (#t: Type)
@@ -231,40 +549,17 @@ fn read
     (i: SZ.t)
     (#p: perm)
     (#s: Ghost.erased (Seq.seq t){SZ.v i < Seq.length s})
-  requires pts_to a #p s
+  preserves pts_to a #p s
   returns res:t
-ensures 
-    pts_to a #p s **
-    pure (res == Seq.index s (SZ.v i))
+  ensures pure (res == Seq.index s (SZ.v i))
 {
   unfold pts_to a #p s;
-  with w. assert (pcm_pts_to (lptr_of a) w);
-  let v = Pulse.Lib.Core.read (lptr_of a) w (fun _ -> w);
-  fold (pts_to a #p s);
-  fst (Some?.v (FStar.Map.sel v ((ptr_of a).offset + SZ.v i)));
+  let res = mask_read a i;
+  fold pts_to a #p s;
+  res
 }
 
 let op_Array_Access = read
-
-let mk_carrier_upd
-  (#elt: Type)
-  (len: nat)
-  (offset: nat)
-  (s: Seq.seq elt)
-  (i: nat)
-  (v: elt)
-  (_: squash (
-    offset + Seq.length s <= len /\
-    i < Seq.length s
-  ))
-: Lemma
-  (ensures (
-    let o = mk_carrier len offset s 1.0R in
-    let o' = mk_carrier len offset (Seq.upd s i v) 1.0R in
-    o' `Map.equal` Map.upd o (offset + i) (Some (v, 1.0R))
-  ))
-= ()
-
 
 fn write
     (#t: Type)
@@ -276,78 +571,27 @@ fn write
   ensures pts_to a (Seq.upd s (SZ.v i) v)
 {
   unfold pts_to a #1.0R s;
-  with w. assert (pcm_pts_to (lptr_of a) w);
-  mk_carrier_upd (SZ.v (ptr_of a).base_len) ((ptr_of a).offset) s (SZ.v i) v ();
-  Pulse.Lib.Core.write (lptr_of a) w _
-      (PM.lift_frame_preserving_upd
-        _ _
-        (Frac.mk_frame_preserving_upd
-          (Seq.index s (SZ.v i))
-          v
-        )
-        _ ((ptr_of a).offset + SZ.v i));
-  fold (pts_to a #1.0R (Seq.upd s (SZ.v i) v));
+  mask_write a i v;
+  fold pts_to a #1.0R (Seq.upd s (SZ.v i) v);
 }
 
 let op_Array_Assignment = write
 
-fn free'
+fn free
     (#elt: Type)
     (a: array elt)
     (#s: Ghost.erased (Seq.seq elt))
-requires
-  pts_to a s **
-  pure (is_full_array a)
-ensures 
-  emp
+  requires pts_to a s
+  requires pure (is_full_array a)
 {
   unfold pts_to a #1.0R s;
+  unfold pts_to_mask a #1.0R s (fun _ -> True);
   with w. assert (pcm_pts_to (lptr_of a) w);
-  // Pulse.Lib.Core.write (ptr_of a).base w (PA.one #elt #(length a)) (frame_preserving_upd_one #elt (length a) s);
   drop_ (pcm_pts_to (lptr_of a) _)
 }
 
-let free = free'
-
-let valid_sum_perm
-  (len: nat)
-  (offset: nat)
-  (slice_len: nat)
-  (p1 p2: perm)
-: Tot prop
-= let open FStar.Real in
-  valid_perm len offset slice_len (p1 +. p2)
-
-
 ghost
-fn mk_carrier_share
-  (#elt: Type u#1)
-  (len: nat)
-  (offset: nat)
-  (s: Seq.seq elt)
-  (p1 p2: perm)
-  (_:squash (valid_sum_perm len offset (Seq.length s) p1 p2))
-  requires emp
-ensures 
-(
-  // let c1 = (mk_carrier len offset s p1) in
-  pure (
-    composable (mk_carrier len offset s p1)
-               (mk_carrier len offset s p2) /\
-    mk_carrier len offset s (p1 +. p2) 
-      `Map.equal` 
-    ((mk_carrier len offset s p1) `compose` (mk_carrier len offset s p2))
-  )
-)
-  
-{
-  ()
-}
-
-
-
-ghost
-fn share'
+fn share
   (#elt:Type)
   (arr:array elt)
   (#s:Ghost.erased (Seq.seq elt))
@@ -356,79 +600,10 @@ fn share'
   ensures pts_to arr #(p /. 2.0R) s ** pts_to arr #(p /. 2.0R) s
 {
   unfold pts_to arr #p s;
-  with w. assert (pcm_pts_to (lptr_of arr) w);
-  mk_carrier_share (SZ.v (ptr_of arr).base_len)
-       (ptr_of arr).offset
-       s
-       (p /. 2.0R) 
-       (p /. 2.0R) ();
-  Pulse.Lib.Core.share (lptr_of arr)
-    (mk_carrier (SZ.v (ptr_of arr).base_len) (ptr_of arr).offset s (p /. 2.0R))
-    (mk_carrier (SZ.v (ptr_of arr).base_len) (ptr_of arr).offset s (p /. 2.0R));
+  mask_share arr;
   fold pts_to arr #(p /. 2.0R) s;
   fold pts_to arr #(p /. 2.0R) s;
 }
-
-let share = share'
-
-let mk_carrier_gather
-  (#elt: Type)
-  (len: nat)
-  (offset: nat)
-  (s1 s2: Seq.seq elt)
-  (p1 p2: perm)
-  (_:squash (
-    let c1 = mk_carrier len offset s1 p1 in
-    let c2 = mk_carrier len offset s2 p2 in
-    composable c1 c2 /\
-    Seq.length s1 == Seq.length s2 /\
-    offset + Seq.length s1 <= len
-  ))
-: squash (
-    let c1 = mk_carrier len offset s1 p1 in
-    let c2 = mk_carrier len offset s2 p2 in
-      composable c1 c2 /\
-      mk_carrier len offset s1 (p1 +. p2) == (c1 `compose` c2) /\
-      mk_carrier len offset s2 (p1 +. p2) == (c1 `compose` c2) /\
-      s1 == s2
-  )
-=
-  let c1 = mk_carrier len offset s1 p1 in
-  let c2 = mk_carrier len offset s2 p2 in
-  assert (composable c1 c2);
-  assert (mk_carrier len offset s1 (p1 +. p2) `Map.equal` (c1 `compose` c2));
-  assert (mk_carrier len offset s2 (p1 +. p2) `Map.equal` (c1 `compose` c2));
-  mk_carrier_inj len offset s1 s2 (p1 +. p2) (p1 +. p2)
-
-
-let mk_carrier_valid_sum_perm
-  (#elt: Type)
-  (len: nat)
-  (offset: nat)
-  (s: Seq.seq elt)
-  (p1 p2: perm)
-: squash
-  (let c1 = mk_carrier len offset s p1 in
-   let c2 = mk_carrier len offset s p2 in
-   composable c1 c2 <==> valid_sum_perm len offset (Seq.length s) p1 p2)
-= let c1 = mk_carrier len offset s p1 in
-  let c2 = mk_carrier len offset s p2 in
-  if Seq.length s > 0 && offset + Seq.length s <= len
-  then
-    let open FStar.Real in
-    assert (Frac.composable (Map.sel c1 offset) (Map.sel c2 offset) <==> valid_perm len offset (Seq.length s) (p1 +. p2))
-  else ()
-
-
-ghost
-fn of_squash (#p:prop) (s:squash p)
-  requires emp
-  ensures pure p
-{
-  ()
-}
-
-
 
 [@@allow_ambiguous]
 ghost
@@ -441,12 +616,10 @@ fn gather
   ensures pts_to arr #(p0 +. p1) s0 ** pure (s0 == s1)
 {
   unfold pts_to arr #p0 s0;
-  with w0. assert (pcm_pts_to (lptr_of arr) w0);
   unfold pts_to arr #p1 s1;
-  with w1. assert (pcm_pts_to (lptr_of arr) w0 ** pcm_pts_to (lptr_of arr) w1);
-  Pulse.Lib.Core.gather (lptr_of arr) w0 w1;
-  of_squash (mk_carrier_gather (SZ.v (ptr_of arr).base_len) ((ptr_of arr).offset) s0 s1 p0 p1 ());
-  of_squash (mk_carrier_valid_sum_perm (SZ.v (ptr_of arr).base_len) ((ptr_of arr).offset) s0 p0 p1);
+  mask_gather arr;
+  with v. assert pts_to_mask arr #(p0 +. p1) v (fun _ -> True);
+  assert pure (v `Seq.equal` s1 /\ v `Seq.equal` s0);
   fold pts_to arr #(p0 +. p1) s0;
 }
 
@@ -463,10 +636,8 @@ fn pts_to_injective_eq
 {
   unfold pts_to arr #p0 s0;
   unfold pts_to arr #p1 s1;
-  Pulse.Lib.Core.gather (lptr_of arr) _ _;
-  Pulse.Lib.Core.share (lptr_of arr) _ _;
-  of_squash (mk_carrier_gather (SZ.v (ptr_of arr).base_len) ((ptr_of arr).offset) s0 s1 p0 p1 ());
-  of_squash (mk_carrier_valid_sum_perm (SZ.v (ptr_of arr).base_len) ((ptr_of arr).offset) s0 p0 p1);
+  pts_to_mask_injective_eq arr;
+  assert pure (Seq.equal s0 s1);
   fold pts_to arr #p0 s0;
   fold pts_to arr #p1 s1;
 }
@@ -478,68 +649,11 @@ fn pts_to_perm_bound (#a:_) (#p:_) (arr: array a) (#s:Seq.seq a)
   ensures pure (p <=. 1.0R)
 {
   unfold pts_to arr #p s;
+  pts_to_mask_props arr;
   fold pts_to arr #p s;
 }
 
-let ptr_shift
-  (p: ptr)
-  (off: nat {offset p + off <= base_len (base p)})
-: ptr
-= {
-    base_len = p.base_len;
-    base = p.base;
-    offset = p.offset + off;
-  }
-
-let split_l'
-    (#elt: Type)
-    (a: array elt)
-    (i: erased nat {i <= length a})
-: array elt
-= { p = ptr_of a; length=i }
-
-irreducible
-let split_l
-  (#elt: Type)
-  (a: array elt)
-  (i: erased nat {i <= length a})
-: x:array elt { x == split_l' a i }
-= split_l' a i
-
-let split_r'
-  (#elt: Type)
-  (a: array elt)
-  (i: nat {i <= length a})
-: array elt
-= { p= ptr_shift (ptr_of a) i; length=Ghost.hide (length a - i) }
-
-irreducible
-let split_r
-  (#elt: Type)
-  (a: array elt)
-  (i: nat {i <= length a})
-: x:array elt { x == split_r' a i }
-= split_r' a i
-
-let array_slice
-  (#elt: Type)
-  (a: array elt)
-  (i:nat) (j: nat {i <= j /\ j <= length a})
-: GTot (array elt)
-= split_l (split_r a i) (j - i)
-
-let in_bounds (i j:nat) (s:array 'a) = squash (i <= j /\ j <= length s)
-
-ghost
-fn elim_in_bounds (#elt:Type) (#i #j:nat) (s:array elt) (p:in_bounds i j s)
-  requires emp
-  ensures pure (i <= j /\ j <= length s)
-{
-  ()
-}
-
-
-let token ([@@@mkey] k:'k) (x:'a) = emp
+open Pulse.Lib.WithPure
 
 let pts_to_range
   (#a:Type)
@@ -548,23 +662,37 @@ let pts_to_range
   (#[exact (`1.0R)] p:perm)
   (s : Seq.seq a)
 : slprop
-= exists* (q:in_bounds i j x). pts_to (array_slice x i j) #p s ** token x q
+= with_pure (i <= j /\ j <= length x) fun _ -> pts_to (gsub x i j) #p s
+
+ghost fn fold_pts_to_range #a (x: array a) (i: nat) (j: nat { i <= j /\ j <= length x }) #p s #mask
+  requires pts_to_mask (gsub x i j) #p s mask
+  requires pure (forall (k: nat). k < j - i ==> mask k)
+  ensures pts_to_range x i j #p s
+{
+  pts_to_mask_props (gsub x i j);
+  mask_mext (gsub x i j) (fun _ -> True);
+  fold pts_to (gsub x i j) #p s;
+  intro_with_pure (i <= j /\ j <= length x) (fun _ -> pts_to (gsub x i j) #p s) ();
+  fold pts_to_range x i j #p s;
+}
+
+ghost fn unfold_pts_to_range #a (x: array a) (i j: nat) #p s
+  requires pts_to_range x i j #p s
+  returns _: squash (i <= j /\ j <= length x)
+  ensures pts_to_mask (gsub x i j) #p s (fun _ -> True)
+{
+  unfold pts_to_range x i j #p s;
+  elim_with_pure (i <= j /\ j <= length x) (fun _ -> pts_to (gsub x i j) #p s);
+  unfold pts_to (gsub x i j) #p s;
+}
 
 let pts_to_range_timeless (#a:Type) (x:array a) (i j : nat) (p:perm) (s:Seq.seq a)
   : Lemma (timeless (pts_to_range x i j #p s))
           [SMTPat (timeless (pts_to_range x i j #p s))]
-  =
-    let aux (q:in_bounds i j x)
-      : Lemma (timeless (pts_to (array_slice x i j) #p s ** token x q))
-    = ()
-    in
-    Classical.forall_intro aux;
-    assert_norm (pts_to_range x i j #p s == (exists* (q:in_bounds i j x). pts_to (array_slice x i j) #p s ** token x q));
-    timeless_exists (fun (q: in_bounds i j x) -> pts_to (array_slice x i j) #p s ** token x q)
-
+  = ()
 
 ghost
-fn pts_to_range_prop'
+fn pts_to_range_prop
   (#elt: Type)
   (a: array elt)
   (#i #j: nat)
@@ -575,18 +703,13 @@ fn pts_to_range_prop'
       (i <= j /\ j <= length a /\ Seq.length s == j - i)
     )
 {
-  unfold pts_to_range a i j #p s;
-  with q. assert (token #(in_bounds i j a) a q);
-  elim_in_bounds a q;
-  pts_to_len (array_slice a i j);
-  fold pts_to_range a i j #p s;
+  unfold_pts_to_range a i j #p s;
+  pts_to_mask_len (gsub a i j);
+  fold_pts_to_range a i j #p s;
 }
 
-let pts_to_range_prop = pts_to_range_prop'
-
-
 ghost
-fn pts_to_range_intro'
+fn pts_to_range_intro
   (#elt: Type)
   (a: array elt)
   (p: perm)
@@ -594,18 +717,13 @@ fn pts_to_range_intro'
   requires pts_to a #p s
   ensures pts_to_range a 0 (length a) #p s
 {
-  rewrite each a as (array_slice a 0 (length a));
-  let q : in_bounds 0 (length a) a = ();
-  fold (token a q);
-  fold (pts_to_range a 0 (length a) #p s);
+  unfold pts_to a #p s;
+  rewrite each a as gsub a 0 (length a);
+  fold_pts_to_range a 0 (length a) #p s;
 }
 
-let pts_to_range_intro = pts_to_range_intro'
-
-
-
 ghost
-fn pts_to_range_elim'
+fn pts_to_range_elim
   (#elt: Type)
   (a: array elt)
   (p: perm)
@@ -613,112 +731,10 @@ fn pts_to_range_elim'
   requires pts_to_range a 0 (length a) #p s
   ensures pts_to a #p s
 {
-  unfold (pts_to_range a 0 (length a) #p s);
-  unfold (token #(in_bounds 0 (length a) a) a _);
-  rewrite each (array_slice a 0 (length a)) as a;
+  unfold_pts_to_range a 0 (length a) #p s;
+  rewrite each gsub a 0 (length a) as a;
+  fold pts_to a #p s;
 }
-
-let pts_to_range_elim = pts_to_range_elim'
-
-let mk_carrier_split
-  (#elt: Type)
-  (len: nat)
-  (offset: nat)
-  (s: Seq.seq elt)
-  (p: perm)
-  (i: nat)
-  (_:squash (
-    offset + Seq.length s <= len /\
-    i <= Seq.length s
-  ))
-: squash (
-    let c1 = mk_carrier len offset (Seq.slice s 0 i) p in
-    let c2 = mk_carrier len (offset + i) (Seq.slice s i (Seq.length s)) p in
-      composable c1 c2 /\
-      mk_carrier len offset s p `Map.equal` (c1 `compose` c2)
-  )
-= ()
-
-
-ghost
-fn use_squash (#p:prop) (s:squash p)
-  requires emp
-  ensures pure p
-{
-  ()
-}
-
-
-
-ghost
-fn ghost_split
-  (#elt: Type)
-  (#x: Seq.seq elt)
-  (#p: perm)
-  (a: array elt)
-  (i: nat {i <= length a})
-  requires pts_to a #p x
-  returns _: squash (i <= length a /\ i <= Seq.length x)
-ensures
-    pts_to (split_r a i) #p (Seq.slice x i (Seq.length x)) **
-    pts_to (split_l a i) #p (Seq.slice x 0 i) **
-    pure (x `Seq.equal` Seq.append (Seq.slice x 0 i) (Seq.slice x i (Seq.length x)))
-{
-  unfold (pts_to a #p x);
-  use_squash (mk_carrier_split (SZ.v (ptr_of a).base_len) (ptr_of a).offset x p i ());
-  let xl = Seq.slice x 0 i;
-  let xr = Seq.slice x i (Seq.length x);
-  let vl = mk_carrier (SZ.v (ptr_of a).base_len) ((ptr_of a).offset) xl p;
-  let vr = mk_carrier (SZ.v (ptr_of a).base_len) ((ptr_of a).offset + i) xr p;
-  Pulse.Lib.Core.share (lptr_of a) vl vr;
-  rewrite pcm_pts_to (lptr_of a) vl
-      as  pcm_pts_to (lptr_of (split_l a i)) vl;
-  rewrite pcm_pts_to (lptr_of a) vr
-      as  pcm_pts_to (lptr_of (split_r a i)) vr;
-  fold (pts_to (split_l a i) #p xl);
-  fold (pts_to (split_r a i) #p xr);
-}
-
-
-let slprop_equiv_refl_eq (v0 v1:slprop) (_:squash (v0 == v1)) : slprop_equiv v0 v1 = 
-  slprop_equiv_refl v0
-
-let equiv () : FStar.Tactics.Tac unit =
-  let open FStar.Tactics in
-  mapply (`slprop_equiv_refl_eq);
-  smt()
-
-
-ghost
-fn split_l_slice #elt
-     (a : array elt)
-     (i m j: nat)
-     (#s:Seq.seq elt)
-     (#p:perm)
-     (_:squash (i <= m /\ m <= j /\ j <= length a))
-  requires pts_to (split_l (array_slice a i j) (m - i)) #p s
-  ensures  pts_to (array_slice a i m) #p s
-{
-  rewrite each (split_l (array_slice a i j) (m - i))
-             as (array_slice a i m);
-}
-
-
-
-ghost
-fn split_r_slice #elt
-     (a:array elt)
-     (i m j: nat)
-     (#s:Seq.seq elt)
-     (#p:perm)
-     (_:squash (i <= m /\ m <= j /\ j <= length a))
-  requires pts_to (split_r (array_slice a i j) (m - i)) #p s
-  ensures pts_to (array_slice a m j) #p s
-{
-  rewrite each (split_r (array_slice a i j) (m - i)) as (array_slice a m j);
-}
-
-
 
 ghost
 fn pts_to_range_split
@@ -742,102 +758,28 @@ ensures
       s == Seq.append s1 s2
     )
 {
-  pts_to_range_prop a;
-  unfold pts_to_range a i j #p s;
-  unfold (token #(in_bounds i j a) a _);
-  ghost_split (array_slice a i j) (m - i);
-  split_r_slice a i m j #(Seq.slice s (m - i) (Seq.length s)) ();
-  split_l_slice a i m j ();
-  let q1 : in_bounds i m a = ();
-  let q2 : in_bounds m j a = ();
-  fold (token #(in_bounds i m a) a q1);
-  fold (token #(in_bounds m j a) a q2);
-  fold (pts_to_range a i m #p (Seq.slice s 0 (m - i)));
-  fold (pts_to_range a m j #p (Seq.slice s (m - i) (Seq.length s)));
-  assert pure (s `Seq.equal` Seq.append (Seq.slice s 0 (m - i)) (Seq.slice s (m - i) (Seq.length s)));
+  unfold_pts_to_range _ _ _ _;
+  pts_to_mask_props (gsub a i j);
+  let s1 = Seq.slice s 0 (m - i);
+  let s2 = Seq.slice s (m - i) (Seq.length s);
+  pcm_share
+    (gsub a i j) p s (fun _ -> True)
+    (gsub a i m) p s1 (fun _ -> True)
+    (gsub a m j) p s2 (fun _ -> True);
+  fold_pts_to_range a i m #p s1;
+  fold_pts_to_range a m j #p s2;
+  assert pure (s `Seq.equal` Seq.append s1 s2);
 }
-
-
-let mk_carrier_merge
-  (#elt: Type)
-  (len: nat)
-  (offset: nat)
-  (s1 s2: Seq.seq elt)
-  (p: perm)
-  (_:squash (
-    offset + Seq.length s1 + Seq.length s2 <= len
-  ))
-: squash (
-    let c1 = mk_carrier len offset s1 p in
-    let c2 = mk_carrier len (offset + Seq.length s1) s2 p in
-      composable c1 c2 /\
-      mk_carrier len offset (s1 `Seq.append` s2) p `Map.equal` (c1 `compose` c2)
-  )
-= ()
 
 let adjacent (#elt: Type) (a1 a2: array elt) : Tot prop =
-  base (ptr_of a1) == base (ptr_of a2) /\
-  offset (ptr_of a1) + (length a1) == offset (ptr_of a2)
+  base_of a1 == base_of a2 /\
+  offset_of a1 + length a1 == offset_of a2
 
-let merge' (#elt: Type) (a1: array elt) (a2:array elt { adjacent a1 a2 })
-= { p = ptr_of a1; length=Ghost.hide (length a1 + length a2) }
-
-irreducible
-let merge #elt (a1:array elt) (a2:array elt{ adjacent a1 a2})
-: i:array elt{ i == merge' a1 a2 } 
-= merge' a1 a2
-
+let merge (#elt: Type) (a1: array elt) (a2:array elt { adjacent a1 a2 }) : array elt
+= { a1 with length = a1.length + a2.length }
 
 ghost
-fn ghost_join
-  (#elt: Type)
-  (#x1 #x2: Seq.seq elt)
-  (#p: perm)
-  (a1 a2: array elt)
-  (h: squash (adjacent a1 a2))
-  requires pts_to a1 #p x1 ** pts_to a2 #p x2
-  ensures pts_to (merge a1 a2) #p (x1 `Seq.append` x2)
-{
-  unfold pts_to a1 #p x1;
-  unfold pts_to a2 #p x2;
-  use_squash (mk_carrier_merge (SZ.v (ptr_of a1).base_len) ((ptr_of a1).offset) x1 x2 p ());
-  with w. rewrite 
-          pcm_pts_to (lptr_of a2) w
-      as  pcm_pts_to (lptr_of a1) (mk_carrier (SZ.v (ptr_of a1).base_len) ((ptr_of a1).offset + Seq.length x1) x2 p);
-  Pulse.Lib.Core.gather (lptr_of a1)
-    (mk_carrier (SZ.v (ptr_of a1).base_len) ((ptr_of a1).offset) x1 (p))
-    (mk_carrier (SZ.v (ptr_of a1).base_len) ((ptr_of a1).offset + Seq.length x1) x2 (p));
-  with w. rewrite
-          pcm_pts_to (lptr_of a1) w
-      as  pcm_pts_to 
-              (lptr_of (merge a1 a2))
-              (mk_carrier (SZ.v (ptr_of (merge a1 a2)).base_len)
-                          ((ptr_of (merge a1 a2)).offset) (x1 `Seq.append` x2) (p));
-  fold (pts_to (merge a1 a2) #p (Seq.append x1 x2));
-}
-
-
-
-ghost
-fn pts_to_range_intro_ij
-  (#elt: Type)
-  (a: array elt)
-  (p: perm)
-  (s: Seq.seq elt)
-  (i j: nat)
-  (_:squash (i <= j /\ j <= length a))
-  requires pts_to (array_slice a i j) #p s
-  ensures pts_to_range a i j #p s
-{
-  let q : in_bounds i j a = ();
-  fold (token #(in_bounds i j a) a q);
-  fold (pts_to_range a i j #p s);
-}
-
-
-
-ghost
-fn pts_to_range_join'
+fn pts_to_range_join
   (#elt: Type)
   (a: array elt)
   (i m j: nat)
@@ -847,30 +789,15 @@ requires
   pts_to_range a i m #p s1 ** pts_to_range a m j #p s2
   ensures pts_to_range a i j #p (s1 `Seq.append` s2)
 {
-  pts_to_range_prop a #i #m;
-  pts_to_range_prop a #m #j;
-  unfold pts_to_range a i m #p s1;
-  unfold token #(in_bounds i m a) a _;
-  unfold pts_to_range a m j #p s2;
-  unfold token #(in_bounds m j a) a _;
-  ghost_join (array_slice a i m) (array_slice a m j) ();
-  rewrite each (merge (array_slice a i m) (array_slice a m j))
-            as (array_slice a i j);
-  pts_to_range_intro_ij a _ _ i j ();
+  unfold_pts_to_range a i m #p s1;
+  unfold_pts_to_range a m j #p s2;
+  gsub_elim a i m;
+  gsub_elim a m j;
+  join_mask a;
+  gsub_intro a i j;
+  mask_ext (gsub a i j) (Seq.append s1 s2) (fun _ -> True);
+  fold_pts_to_range a i j #p (Seq.append s1 s2);
 }
-
-let pts_to_range_join = pts_to_range_join'
-
-irreducible
-let array_slice_impl
-  (#elt: Type)
-  (a: array elt)
-  (i: SZ.t)
-  (j: Ghost.erased nat)
-  (sq: squash (SZ.v i <= j /\ j <= length a))
-: x:array elt { x == array_slice a (SZ.v i) j }
-= split_l (split_r a (SZ.v i)) (Ghost.hide (j - SZ.v i))
-
 
 fn pts_to_range_index
   (#t: Type)
@@ -887,19 +814,14 @@ fn pts_to_range_index
     pure (eq2 #int (Seq.length s) (r - l) /\
           res == Seq.index s (SZ.v i - l))
 {
-  pts_to_range_split a l (SZ.v i) r;
-  with s1 s2. _;
-  unfold pts_to_range a (SZ.v i) r #p s2;
-  unfold (token #(in_bounds (SZ.v i) r a) a _);
-  let a' = array_slice_impl a i r ();
-  rewrite each (array_slice a (SZ.v i) r) as a';
-  let res = read a' 0sz;
-  rewrite each a' as (array_slice a (SZ.v i) r);
-  pts_to_range_intro_ij a _ _ (SZ.v i) r ();
-  pts_to_range_join a l (SZ.v i) r;
+  unfold_pts_to_range a l r #p s;
+  gsub_elim a l r;
+  let res = mask_read a i;
+  gsub_intro a l r;
+  mask_vext (gsub a l r) s;
+  fold_pts_to_range a l r #p s;
   res
 }
-
 
 fn pts_to_range_upd
   (#t: Type)
@@ -918,18 +840,13 @@ fn pts_to_range_upd
           s == Seq.upd s0 (SZ.v i - l) v
       )
 {
-  pts_to_range_split a l (SZ.v i) r;
-  with s1 s2. _;
-  unfold pts_to_range a (SZ.v i) r #1.0R s2;
-  unfold (token #(in_bounds (SZ.v i) r a) a _);
-  let a' = array_slice_impl a i r ();
-  rewrite each (array_slice a (SZ.v i) r) as a';
-  write a' 0sz v;
-  rewrite each a' as (array_slice a (SZ.v i) r);
-  pts_to_range_intro_ij a _ _ (SZ.v i) r ();
-  pts_to_range_join a l (SZ.v i) r;
-  with w. assert (pts_to_range a l r w);
-  assert pure (w `Seq.equal` Seq.upd s0 (SZ.v i - l) v);
+  unfold_pts_to_range a l r #1.0R s0;
+  gsub_elim a l r;
+  mask_write a i v;
+  gsub_intro a l r;
+  let s = hide (Seq.upd s0 (SZ.v i - l) v);
+  mask_vext (gsub a l r) s;
+  fold_pts_to_range a l r #1.0R s;
 }
 
 ghost
@@ -942,12 +859,10 @@ fn pts_to_range_share
       requires pts_to_range arr l r #p s
       ensures pts_to_range arr l r #(p /. 2.0R) s ** pts_to_range arr l r #(p /. 2.0R) s
 {
-  pts_to_range_prop arr;
-  unfold (pts_to_range arr l r #p s);
-  unfold (token #(in_bounds l r arr) arr _);
-  share (array_slice arr l r);
-  pts_to_range_intro_ij arr (p /. 2.0R) s l r ();
-  pts_to_range_intro_ij arr (p /. 2.0R) s l r ();
+  unfold_pts_to_range arr l r #p s;
+  mask_share (gsub arr l r);
+  fold_pts_to_range arr l r s;
+  fold_pts_to_range arr l r s;
 }
 
 ghost
@@ -960,10 +875,10 @@ fn pts_to_range_gather
       requires pts_to_range arr l r #p0 s0 ** pts_to_range arr l r #p1 s1
       ensures pts_to_range arr l r #(p0 +. p1) s0 ** pure (s0 == s1)
 {
-  pts_to_range_prop arr #l #r #p0;
-  unfold (pts_to_range arr l r #p0 s0);
-  unfold (token #(in_bounds l r arr) arr _);
-  unfold (pts_to_range arr l r #p1 s1);
-  gather (array_slice arr l r);
-  fold (pts_to_range arr l r #(p0 +. p1) s0)
+  unfold_pts_to_range arr l r s0;
+  unfold_pts_to_range arr l r s1;
+  mask_gather (gsub arr l r);
+  with s. assert pts_to_mask (gsub arr l r) #(p0 +. p1) s (fun _ -> True);
+  fold_pts_to_range arr l r s;
+  assert pure (Seq.equal s s0 /\ Seq.equal s s1);
 }
